B = \\\begin{pmatrix}\dfrac{\partial }{\partial r } \left( \dfrac{1}{T} \right) v + \dfrac{1}{T} \left(\vec{\nabla} \cdot \vec{v}\right) & - \dfrac{\partial }{\partial r } \left( \dfrac{\rho}{T} \right) v - \dfrac{\rho}{T} \left(\vec{\nabla} \cdot \vec{v}\right) & \dfrac{2}{r} \rho + \rho' & - \dfrac{2}{r} \rho & 0 & 0\\\dfrac{v}{T} v' & - \dfrac{\rho}{T} v v' & \rho v' & 0 & 0 & 0\\\dfrac{1}{\gamma r} & 0 & 0 & \dfrac{\rho}{r} v & 0 & 0\\B_{41} & - \dfrac{v}{2} \dfrac{\partial }{\partial r } \left( \dfrac{\rho v^{2}}{T} \right) - \dfrac{\left(\vec{\nabla} \cdot \vec{v}\right)}{2 T} \rho v^{2} & B_{43} & - \dfrac{2}{r} k & 0 & 0\\\dfrac{\Lambda}{T} \lambda q & - \dfrac{\Lambda}{T} \rho \lambda q & 0 & 0 & \Lambda \rho \lambda & \dfrac{\partial \Lambda}{\partial E } \rho \lambda q\\\dfrac{2}{T} L \lambda & - \dfrac{2}{T} L \rho \lambda & 0 & 0 & 0 & 2 \dfrac{\partial L}{\partial E } \rho \lambda\end{pmatrix}\nonumber ,\displaybreak[0] \\ \text{with} \nonumber \displaybreak[0] \\ 
B_{41} = \dfrac{v}{2} \dfrac{\partial }{\partial r } \left( \dfrac{v^{2}}{T} \right) + \left(\vec{\nabla} \cdot \vec{v}\right) \left(\dfrac{1}{\gamma - 1} + \dfrac{v^{2}}{2 T}\right),\displaybreak[0] \\ 
B_{43} = \dfrac{\partial }{\partial r } \left( \rho v \right) v + \left(\vec{\nabla} \cdot \vec{v}\right) \rho v + \dfrac{2}{r} k + k'