C_{\star11} = \frac{16 \Psi \gamma - \chi^{2} \gamma^{2} - \chi^{2} \gamma + 16 \gamma \lambda - 8 \gamma - 8}{4 \left(\chi \gamma + \chi + 2 \gamma - 6\right)}
\displaybreak[0] \\C_{\star12} = \frac{\gamma \left(- 16 \Psi \chi \gamma - 16 \Psi \chi + 64 \Psi + \chi^{3} \gamma^{2} + 4 \chi^{3} \gamma + \chi^{3} + 8 \chi^{2} \gamma - 12 \chi^{2} - 16 \chi \gamma \lambda + 80 \chi \gamma - 16 \chi \lambda + 64 \gamma + 64 \lambda - 256\right)}{4 \left(\chi^{2} \gamma^{2} + 2 \chi^{2} \gamma + \chi^{2} + 2 \chi \gamma^{2} - 8 \chi \gamma - 10 \chi - 8 \gamma + 24\right)}
\displaybreak[0] \\C_{\star13} = \frac{\gamma \left(- 4 \Psi \chi \gamma - 4 \Psi \chi + 16 \Psi - \chi^{3} \gamma^{2} - 4 \chi^{3} \gamma - \chi^{3} + 4 \chi^{2} \gamma + 12 \chi^{2} - 4 \chi \gamma \lambda + 16 \chi \gamma - 4 \chi \lambda + 24 \chi + 32 \gamma + 16 \lambda - 128\right)}{2 \left(\chi^{2} \gamma^{2} + 2 \chi^{2} \gamma + \chi^{2} + 2 \chi \gamma^{2} - 8 \chi \gamma - 10 \chi - 8 \gamma + 24\right)}
\displaybreak[0] \\C_{\star14} = \frac{\gamma \left(- \chi^{2} \gamma^{2} - \chi^{2} \gamma + 2 \chi^{2} - 8 \chi \gamma - 8 \chi - 16 \gamma + 48\right)}{\chi^{2} \gamma^{2} + 2 \chi^{2} \gamma + \chi^{2} + 2 \chi \gamma^{2} - 8 \chi \gamma - 10 \chi - 8 \gamma + 24}
\displaybreak[0] \\C_{\star15} = \frac{2 \gamma \left(\Psi \chi \gamma + \Psi \chi - 4 \Psi - \chi^{2} \gamma + \chi \gamma \lambda - 8 \chi \gamma + \chi \lambda - 2 \chi - 8 \gamma - 4 \lambda + 32\right)}{\chi^{2} \gamma^{2} + 2 \chi^{2} \gamma + \chi^{2} + 2 \chi \gamma^{2} - 8 \chi \gamma - 10 \chi - 8 \gamma + 24}
\displaybreak[0] \\C_{\star16} = \frac{\gamma \left(- \Psi \chi^{2} \gamma + 2 \Psi \chi \gamma \lambda \left. \frac{d}{d \xi} L \right|_{\substack{ \xi=1 }} + 2 \Psi \chi \gamma \lambda - 8 \Psi \chi \gamma + 2 \Psi \chi \lambda \left. \frac{d}{d \xi} L \right|_{\substack{ \xi=1 }} + 2 \Psi \chi \lambda - 2 \Psi \chi - 8 \Psi \gamma - 8 \Psi \lambda \left. \frac{d}{d \xi} L \right|_{\substack{ \xi=1 }} - 8 \Psi \lambda + 32 \Psi + \Xi \chi \gamma \lambda + \Xi \chi \lambda - 4 \Xi \lambda\right)}{L \lambda \left(\chi^{2} \gamma^{2} + 2 \chi^{2} \gamma + \chi^{2} + 2 \chi \gamma^{2} - 8 \chi \gamma - 10 \chi - 8 \gamma + 24\right)}
\displaybreak[0] \\C_{\star21} = \frac{16 \Psi \gamma^{2} - 16 \Psi \gamma + \chi^{2} \gamma^{3} - \chi^{2} \gamma + 4 \chi \gamma^{3} - 16 \chi \gamma^{2} + 12 \chi \gamma + 16 \gamma^{2} \lambda - 8 \gamma^{2} - 16 \gamma \lambda + 8}{4 \gamma \left(\chi \gamma + \chi + 2 \gamma - 6\right)}
\displaybreak[0] \\C_{\star22} = \frac{- 2 \left(\Psi + \lambda\right) \left(\gamma - 1\right) \left(\chi \left(\gamma + 1\right) - 4\right) - \frac{\left(\chi \gamma + 3 \chi - 8\right) \left(- 8 \Psi + 4 \chi \gamma + 2 \chi \left(\chi \left(\gamma - 1\right) - 4\right) + 4 \chi + 8 \gamma \left(\Psi + \lambda\right) - 8 \lambda + \left(\chi \left(\gamma - 1\right) - 4\right) \left(\chi \left(\gamma - 1\right) + 4 \gamma - 4\right)\right)}{4} + \frac{\left(\chi \gamma - \chi - 2 \gamma + 2\right) \left(8 \Psi + \chi^{2} \gamma + 4 \chi \gamma - 8 \chi + 8 \lambda - 16\right)}{2}}{\chi^{2} \gamma^{2} + 2 \chi^{2} \gamma + \chi^{2} + 2 \chi \gamma^{2} - 8 \chi \gamma - 10 \chi - 8 \gamma + 24}
\displaybreak[0] \\C_{\star23} = \frac{\left(\chi \gamma + 3 \chi - 8\right) \left(- 4 \Psi \gamma + 4 \Psi - \chi^{2} \gamma^{2} + \chi^{2} \gamma + 2 \chi \gamma - 6 \chi - 4 \gamma \lambda + 4 \lambda + 8\right) + \left(\chi \gamma - \chi - 2 \gamma + 2\right) \left(8 \Psi + \chi^{2} \gamma + \chi^{2} - 8 \chi + 8 \lambda\right)}{2 \left(\chi^{2} \gamma^{2} + 2 \chi^{2} \gamma + \chi^{2} + 2 \chi \gamma^{2} - 8 \chi \gamma - 10 \chi - 8 \gamma + 24\right)}
\displaybreak[0] \\C_{\star24} = \frac{\chi \left(- \chi \gamma^{3} + 2 \chi \gamma^{2} + 3 \chi \gamma - 4 \chi + 4 \gamma^{2} - 16 \gamma + 12\right)}{\chi^{2} \gamma^{2} + 2 \chi^{2} \gamma + \chi^{2} + 2 \chi \gamma^{2} - 8 \chi \gamma - 10 \chi - 8 \gamma + 24}
\displaybreak[0] \\C_{\star25} = \frac{2 \left(- 2 \Psi \left(\chi \gamma - \chi - 2 \gamma + 2\right) + \lambda \left(\gamma - 1\right) \left(\chi \gamma + \chi - 4\right) + \left(\chi \gamma + 3 \chi - 8\right) \left(\Psi \gamma - \Psi + \chi \gamma - 2\right)\right)}{\chi^{2} \gamma^{2} + 2 \chi^{2} \gamma + \chi^{2} + 2 \chi \gamma^{2} - 8 \chi \gamma - 10 \chi - 8 \gamma + 24}
\displaybreak[0] \\C_{\star26} = \frac{\lambda \left(2 \Psi \left(\gamma - 1\right) \left(\chi \gamma + \chi - 4\right) \left. \frac{d}{d \xi} L \right|_{\substack{ \xi=1 }} + \Psi \left(\gamma - 1\right) \left(\chi \gamma + \chi - 4\right) - 2 \left(\Psi + \Xi\right) \left(\chi \gamma - \chi - 2 \gamma + 2\right)\right) - \frac{\left(\Psi \left(\chi \left(\gamma - 1\right) - \chi \left(3 \gamma - 1\right) + 4\right) - 2 \lambda \left(\Psi + \Xi\right) \left(\gamma - 1\right)\right) \left(\chi \gamma + 3 \chi - 8\right)}{2}}{L \lambda \left(\chi^{2} \gamma^{2} + 2 \chi^{2} \gamma + \chi^{2} + 2 \chi \gamma^{2} - 8 \chi \gamma - 10 \chi - 8 \gamma + 24\right)}
\displaybreak[0] \\C_{\star31} = \frac{- 16 \Psi \gamma - \chi^{2} \gamma^{2} - \chi^{2} \gamma - 4 \chi \gamma^{2} + 12 \chi \gamma - 16 \gamma \lambda + 8 \gamma + 8}{4 \gamma \left(\chi \gamma + \chi + 2 \gamma - 6\right)}
\displaybreak[0] \\C_{\star32} = \frac{4 \Psi \chi \gamma + 4 \Psi \chi - 16 \Psi + \frac{\chi^{3} \gamma^{2}}{4} + \frac{\chi^{3}}{4} + \chi^{2} \gamma^{2} - 4 \chi^{2} \gamma + 4 \chi \gamma \lambda - 12 \chi \gamma + 4 \chi \lambda + 8 \chi - 16 \lambda + 16}{\chi^{2} \gamma^{2} + 2 \chi^{2} \gamma + \chi^{2} + 2 \chi \gamma^{2} - 8 \chi \gamma - 10 \chi - 8 \gamma + 24}
\displaybreak[0] \\C_{\star33} = \frac{2 \Psi \chi \gamma + 2 \Psi \chi - 8 \Psi + \chi^{3} \gamma - \chi^{2} \gamma^{2} - 2 \chi^{2} \gamma - 5 \chi^{2} + 2 \chi \gamma \lambda - 4 \chi \gamma + 2 \chi \lambda + 8 \chi - 8 \lambda + 16}{\chi^{2} \gamma^{2} + 2 \chi^{2} \gamma + \chi^{2} + 2 \chi \gamma^{2} - 8 \chi \gamma - 10 \chi - 8 \gamma + 24}
\displaybreak[0] \\C_{\star34} = \frac{\chi^{2} \left(\gamma^{2} + \gamma - 2\right)}{\chi^{2} \gamma^{2} + 2 \chi^{2} \gamma + \chi^{2} + 2 \chi \gamma^{2} - 8 \chi \gamma - 10 \chi - 8 \gamma + 24}
\displaybreak[0] \\C_{\star35} = \frac{2 \left(- 2 \Psi \left(\chi \gamma + 2 \gamma - 4\right) - \lambda \left(\chi \gamma + \chi - 4\right) + \left(\chi + 4\right) \left(\Psi \gamma - \Psi + \chi \gamma - 2\right)\right)}{\chi^{2} \gamma^{2} + 2 \chi^{2} \gamma + \chi^{2} + 2 \chi \gamma^{2} - 8 \chi \gamma - 10 \chi - 8 \gamma + 24}
\displaybreak[0] \\C_{\star36} = \frac{\lambda \left(- 2 \Psi \left(\chi \gamma + \chi - 4\right) \left. \frac{d}{d \xi} L \right|_{\substack{ \xi=1 }} - \Psi \left(\chi \gamma + \chi - 4\right) - 2 \left(\Psi + \Xi\right) \left(\chi \gamma + 2 \gamma - 4\right)\right) - \frac{\left(\chi + 4\right) \left(\Psi \left(\chi \left(\gamma - 1\right) - \chi \left(3 \gamma - 1\right) + 4\right) - 2 \lambda \left(\Psi + \Xi\right) \left(\gamma - 1\right)\right)}{2}}{L \lambda \left(\chi^{2} \gamma^{2} + 2 \chi^{2} \gamma + \chi^{2} + 2 \chi \gamma^{2} - 8 \chi \gamma - 10 \chi - 8 \gamma + 24\right)}
\displaybreak[0] \\C_{\star(4-6)(1-6)} = \left[\begin{matrix}- \frac{1}{\gamma} & 0 & 0 & -1 & 0 & 0\\\lambda & - \lambda & 0 & 0 & \lambda & \frac{\Psi}{2 L}\\2 L \lambda & - 2 L \lambda & 0 & 0 & 0 & 2 \lambda \left. \frac{d}{d \xi} L \right|_{\substack{ \xi=1 }}\end{matrix}\right]